PF3-3 Dafny proofs

PF3-3/exam3-2025/problem5/sol5.dfy
@@ -14,20 +14,20 @@ method factorial(n: nat) returns (f: nat)
   ensures f == fac(n)
 {
   f := 1;
-  var i := 1;
-  
-  while (i <= n)
-    invariant 1 <= i <= n + 1 && f == fac(i - 1)
-  {
-    var v, j := f, 0;
+  var i: nat := 0;
 
-    while (j < i - 1)
-      invariant 0 <= j <= i - 1 && f == v + j * fac(i - 1)
+  while i < n
+    invariant 0 <= i <= n && f == fac(i)
+  {
+    var v, j: nat := f, 0;
+
+    while j < i
+      invariant 0 <= j <= i && f == v + j * v
     {
       f := f + v;
       j := j + 1;
     }
-
-    i := i + 1;
+    
+    i := i + 1;       
   }
 }
